Makefile
@@ -58,7 +58,7 @@ FLOCQ=\
 VLIB=Axioms.v Coqlib.v Intv.v Maps.v Heaps.v Lattice.v Ordered.v \
   Iteration.v Integers.v Archi.v Fappli_IEEE_extra.v Floats.v \
   Parmov.v UnionFind.v Wfsimpl.v \
-  Postorder.v FSetAVLplus.v IntvSets.v Decidableplus.v
+  Postorder.v FSetAVLplus.v IntvSets.v Decidableplus.v BoolEqual.v
 
 # Parts common to the front-ends and the back-end (in common/)
 
